examples for c-extraction

examples/low-star/test2.c
@@ -1,0 +1,51 @@
+#include<stdio.h>
+#include<stdlib.h>
+#include<unistd.h>
+
+#define MAX_LENGTH 25
+
+// F* -> C generated code
+extern void Ex2_process_msg(char* buffer);
+
+// Expects a valid file name as input
+// Encrypt and decrypt its content on the fly
+int main(int argc, char **argv){
+  char *mod = "r+";
+  int size_read, fd;
+  char msg[MAX_LENGTH + 3];
+  FILE *file;
+
+  file = fopen(argv[1],mod);
+
+  if (file == NULL){
+    printf("ERROR : Cannot open input file");
+    exit(1);
+  }
+
+  fd = fileno(file);
+
+  // Fill msg buffer with at most 25 characters of the input file
+  size_read = read(fd, (msg+2), MAX_LENGTH);
+  
+  if (size_read == -1){
+    printf("ERROR : Cannot read input file");
+    exit(1);
+  }
+
+  // Set the msg size
+  msg[0] = size_read;
+  msg[1] = 0;
+
+  // Call encryption function
+  Ex2_process_msg(msg);
+  // Print result
+  printf("After first encryption : %s\n\n", msg+2);
+  // Call decryption function
+  Ex2_process_msg(msg);
+  // Print result
+  printf("After second encryption : %s\n\n", msg+2);
+
+  // Close fd and exit
+  fclose(file);
+  return 0;
+}
