examples/low-star/ex2.fst
@@ -1,0 +1,86 @@
+(*--build-config
+  options:--admit_fsi FStar.Set --admit_fsi FStar.Seq --verify_module Ex2 --z3timeout 10 --codegen C;
+  variables:SST=../low-level;
+  other-files:classical.fst ext.fst set.fsi seq.fsi seqproperties.fst heap.fst st.fst all.fst list.fst listTot.fst listproperties.fst $SST/stack.fst $SST/listset.fst ghost.fst $SST/located.fst $SST/lref.fst $SST/regions.fst $SST/rst.fst $SST/sstCombinators.fst lsarray.fst
+  --*)
+
+
+module Ex2
+
+(* Demonstrates the C generation for F* *)
+
+open RST
+open Located
+open Lref
+open FStar.Set
+open FStar.Ghost
+open Regions
+open Stack
+open RSTCombinators
+open LSarray
+
+(* Custom char type, for simplicity *)
+type char = b:nat{ b < 256 }
+
+(* Mimics encrytion : xor the buffer's content with 42 *)
+val encrypt:
+  buffer:LSarray.array char -> len:nat ->
+  Mem 
+    unit
+    (requires (fun m -> 
+      (isNonEmpty (st m))
+      /\ (live buffer m)
+      /\ (len <= glength buffer)))
+    (ensures (fun m0 _ m1 ->
+      (isNonEmpty (st m0))
+      /\ (isNonEmpty (st m1))
+      /\ (live buffer m0)
+      /\ (live buffer m1)
+      /\ (len <= glength buffer)
+      /\ (forall (i:nat{ i < len }). gget buffer i m1 = op_Hat_Bar (gget buffer i m0) 42)))
+    (eonly (asRef buffer))
+let encrypt buffer len =
+  let m_init = RST.get() in
+  pushRegion();
+  let ctr = ralloc #nat 0 in
+  scopedWhile1 ctr 
+	      (fun ctr -> ctr < len) 
+	      (fun m -> 
+		(isNonEmpty (st m))
+		/\ (refIsLive ctr m)
+		/\ (live buffer m)
+		/\ (lookupRef ctr m <= len)
+		/\ (forall (i:nat{ i < lookupRef ctr m }). gget buffer i m = op_Hat_Bar (gget buffer i (reveal m_init)) 42 )
+		/\ (forall (i:nat{ i >= lookupRef ctr m /\ i < len }). gget buffer i m = gget buffer i (reveal m_init)))
+	      (eunion (only ctr) (eonly (asRef buffer)))
+	      (fun (u:unit) ->
+		let idx = memread ctr in
+		let v = LSarray.get buffer idx in
+		let v2 = v ^| 42 in // Symbolizes the xor operator
+		LSarray.upd buffer idx v2;
+		memwrite ctr (idx + 1)
+		);
+  let m = RST.get() in
+  popRegion()
+
+(* Safety check : well formedness of the initial buffer received *)
+type wellFormed (m:smem) (buffer:LSarray.array char) =
+  (live buffer m)
+  /\ (glength buffer >= 2)
+  /\ (glength buffer >= (gget buffer 0 m + 256 * (gget buffer 1 m)) + 2) 
+
+(* Reads lengths of msg, and proceeds to its encryption *)
+val process_msg:
+  buffer:LSarray.array char -> 
+  Mem unit
+    (requires (fun m -> 
+      (isNonEmpty (st m))
+      /\ (wellFormed m buffer)))
+    (ensures (fun m0 _ m1 -> True))
+    (eonly (asRef buffer))
+let process_msg buffer =
+  let l0 = get buffer 0 in
+  let l1 = get buffer 1 in
+  let len = l0 + 256 * l1 in
+  let msg_body = sub buffer 2 len in
+  encrypt msg_body len
